common/dnf.lean
@@ -2,6 +2,8 @@ import .atom
 
 variables {α β : Type}
 
+open atom_type
+
 /-
 Requires : nqfree arg-0
 -/
@@ -11,15 +13,53 @@ def dnf : fm α → list (list α)
 | (fm.atom a) := [[a]]
 | (fm.and p q) := list.map append_pair $ list.product (dnf p) (dnf q)
 | (fm.or p q) := dnf p ++ dnf q 
-| _ := []
+| (fm.ex _) := []
+| (fm.not _) := []
 
-lemma dnf_prsv [atom_type α β] {p : fm α} {H : nqfree p} {bs : list β} : 
-  some_true (list.map (allp (atom_type.val bs)) (dnf p)) ↔ I p bs := sorry
--- iff.trans (by rewrite some_true_iff_disj_list) (dnf_prsv _ H _)
+lemma dnf_prsv_normal [atom_type α β] : ∀ (p : fm α), 
+  fnormal β p → allp (allp (normal β)) (dnf p) 
+| (fm.true α) hnm := 
+  begin
+    intros as has, unfold dnf at has,
+    rewrite exp_mem_singleton at has, subst has,
+    apply allp_nil
+  end
+| (fm.false α) hnm := allp_nil
+| (fm.atom a) hnm := 
+  begin
+    intros as has, unfold dnf at has,
+    rewrite exp_mem_singleton at has, 
+    subst has, intros a' ha', 
+    rewrite exp_mem_singleton at ha',
+    subst ha', apply hnm,
+  end
+| (fm.and p q) hnm := 
+  begin
+    unfold fnormal at hnm, cases hnm with hnmp hnmq,
+    unfold dnf, intros as has, intros a ha,
+    rewrite exp_mem_map at has, 
+    cases has with asp hasp, 
+    cases hasp with hasp1 hasp2,
+    cases asp with as1 as2, subst hasp2, 
+    cases (mem_or_mem_of_mem_append ha) with hm hm,
+    apply dnf_prsv_normal p hnmp as1, 
+    apply fst_mem_of_mem_product hasp1, apply hm,  
+    apply dnf_prsv_normal q hnmq as2, 
+    apply snd_mem_of_mem_product hasp1, apply hm
+  end
+| (fm.or p q) hnm := 
+  begin
+    unfold fnormal at hnm, cases hnm with hnmp hnmq,
+    unfold dnf, intros as has, intros a ha,
+    cases (mem_or_mem_of_mem_append has) with hm hm,
+    apply dnf_prsv_normal p hnmp as hm a ha, 
+    apply dnf_prsv_normal q hnmq as hm a ha 
+  end
+| (fm.not _) hnm := allp_nil
+| (fm.ex _) hnm := allp_nil
 
-#exit
-lemma dnf_prsv [atom_type α β] : ∀ (p : fm α) (H : nqfree p) (xs : list β), 
-  disj_list (list.map (λ (as : list α), allp (atom_type.val xs) as) (dnf p)) ↔ I p xs 
+lemma dnf_prsv_alt [atom_type α β] : ∀ {p : fm α} {H : nqfree p} {xs : list β}, 
+  disj_list (list.map (allp (atom_type.val xs)) (dnf p)) ↔ I p xs 
 | (fm.true α) H bs := 
   by {unfold dnf, simp, unfold disj_list, 
       rewrite exp_allp_nil, rewrite true_or,
@@ -37,8 +77,8 @@ lemma dnf_prsv [atom_type α β] : ∀ (p : fm α) (H : nqfree p) (xs : list β)
 | (fm.and p q) H bs := 
   begin
     unfold dnf, rewrite map_compose, rewrite exp_I_and, 
-    rewrite (iff.symm (dnf_prsv p H^.elim_left bs)),
-    rewrite (iff.symm (dnf_prsv q H^.elim_right bs)),
+    rewrite iff.symm (@dnf_prsv_alt p _ bs),
+    rewrite iff.symm (@dnf_prsv_alt q _ bs),
     repeat {rewrite disj_list_iff_some_true},
     repeat {unfold some_true},
 
@@ -50,7 +90,7 @@ lemma dnf_prsv [atom_type α β] : ∀ (p : fm α) (H : nqfree p) (xs : list β)
     simp at Hd, 
     apply and.intro, 
          
-    existsi (∀ (a : α), a ∈ (prod.fst d) → atom_type.val a bs),
+    existsi (∀ (a : α), a ∈ (prod.fst d) → atom_type.val bs a),
     apply and.intro, apply mem_map_of_mem,
     apply fst_mem_of_mem_product Hd^.elim_right,
     intros a Ha, rewrite Hd^.elim_left at Hrr,
@@ -58,7 +98,7 @@ lemma dnf_prsv [atom_type α β] : ∀ (p : fm α) (H : nqfree p) (xs : list β)
     apply mem_append_of_mem_or_mem,
     apply or.inl Ha, 
 
-    existsi (∀ (a : α), a ∈ (prod.snd d) → atom_type.val a bs),
+    existsi (∀ (a : α), a ∈ (prod.snd d) → atom_type.val bs a),
     apply and.intro, apply mem_map_of_mem, 
     apply snd_mem_of_mem_product Hd^.elim_right,
     intros a Ha, rewrite Hd^.elim_left at Hrr,
@@ -71,7 +111,7 @@ lemma dnf_prsv [atom_type α β] : ∀ (p : fm α) (H : nqfree p) (xs : list β)
     cases (H0^.elim_right) with s Hs, clear H0, 
     cases (ex_arg_of_mem_map Hr^.elim_left) with ll Hll,
     cases (ex_arg_of_mem_map Hs^.elim_left) with lr Hlr,
-    existsi (∀ (a : α), a ∈ append_pair (ll,lr) → atom_type.val a bs),
+    existsi (∀ (a : α), a ∈ append_pair (ll,lr) → atom_type.val bs a),
     apply and.intro, apply mem_map_of_mem, 
     apply mem_product_of_mem_of_mem,
     apply Hll^.elim_left, apply Hlr^.elim_left,
@@ -80,15 +120,20 @@ lemma dnf_prsv [atom_type α β] : ∀ (p : fm α) (H : nqfree p) (xs : list β)
     rewrite Hll^.elim_right at Hr,
     apply Hr^.elim_right _ HM, 
     rewrite Hlr^.elim_right at Hs,
-    apply Hs^.elim_right _ HM 
+    apply Hs^.elim_right _ HM,
+    apply H^.elim_right, apply H^.elim_left
   end
 | (fm.or p q) H bs := 
   begin
     unfold dnf, rewrite map_dist_append, 
     rewrite disj_list_dist_append,
-    rewrite dnf_prsv, rewrite dnf_prsv,
+    rewrite dnf_prsv_alt, rewrite dnf_prsv_alt,
     rewrite exp_I_or, apply H^.elim_right,
     apply H^.elim_left
   end
 | (fm.not p) H bs := by cases H
 | (fm.ex p) H bs := by cases H
+
+lemma dnf_prsv [atom_type α β] {p : fm α} {H : nqfree p} {bs : list β} : 
+  some_true (list.map (allp (atom_type.val bs)) (dnf p)) ↔ I p bs := 
+iff.trans (by rewrite some_true_iff_disj_list) (@dnf_prsv_alt _ _ _ _ H _)
