common/ldq.lean
@@ -4,88 +4,6 @@ variables {α β : Type}
 
 open atom_type
 
-def qe_prsv (β : Type) [atom_type α β] (qe : list α → fm α) (as : list α) : Prop := 
-  ∀ (bs : list β), ((I (qe as) bs) ↔ (∃ x, allp (val (x::bs)) as))
-
-/- 
-Requires : qe takes a list of atoms that are all dependent on 0-variable,
-  and returns formula which (1) does not contain the 0-variable, and 
-  (2) is equivalent to the conjunction of input list.
--/
-def qelim (β) [atom_type α β] (qe : list α → fm α) (as : list α) : fm α :=
-  and_o 
-    (qe (@list.filter _ (dep0 β) (dec_dep0 _ _) as)) 
-    (list_conj (list.map (λ (a : α), A' (decr β a)) (@list.filter _ (λ a, ¬ (dep0 β a)) 
-      (begin 
-         intro a, cases (dec_dep0 _ _ a) with H H, 
-         apply decidable.is_true H, 
-         apply decidable.is_false (not_not_intro H)
-       end) as)))
-      
-      #check exp_I_list_conj
-lemma qelim_prsv [atom_type α β] {r} {qe} 
-  (hqe : ∀ as, allp (dep0 β) as → allp r as → qe_prsv β qe as)
-  {as : list α} (bs : list β) : 
-  (I (qelim β qe as) bs) ↔ (∃ b, allp (val (b::bs)) as) := 
-begin
-  apply iff.intro; intro h,
-  unfold qelim at h, 
-  rewrite exp_I_and_o at h, cases h with h1 h2,
-  rewrite hqe at h1, cases h1 with b h1, 
-  existsi b, intros a ha,
-  cases (atom_type.dec_dep0 _ β a),
-  rewrite exp_I_list_conj at h2, 
-
-end
-
-def lift_dnf_qe (β : Type) [atom_type α β] (qe : list α → fm α) : fm α → fm α 
-| (fm.true α) := ⊤'
-| (fm.false α) := ⊥'
-| (fm.atom a) := A' a
-| (fm.and p q) := (lift_dnf_qe p) ∧' (lift_dnf_qe q)
-| (fm.or p q) := (lift_dnf_qe p) ∨' (lift_dnf_qe q)
-| (fm.not p) := ¬' (lift_dnf_qe p) 
-| (fm.ex p) := dnf_to_fm (dnf (@nnf _ β _ $ lift_dnf_qe p)) (@qelim _ β _ @qe)
-
-lemma atoms_conj_qfree [atom_type α β] : ∀ (as : list α), qfree (list_conj (list.map (λ (a : α), A' decr β a) as )) 
-| [] := trivial
-| (a::as) := 
-  begin 
-    unfold list.map, unfold list_conj, 
-    apply cases_and_o, trivial, trivial,
-    apply atoms_conj_qfree, unfold qfree, 
-    apply and.intro trivial,
-    apply atoms_conj_qfree
-  end
-
-lemma ldq_qfree [atom_type α β] (qe : list α → fm α)  
-  (H : ∀ (l : list α), allp (dep0 β) l → qfree (qe l)) :
-  ∀ (p : fm α), qfree (lift_dnf_qe β qe p)  
-| (fm.true α) := trivial
-| (fm.false α) := trivial
-| (fm.atom a) := trivial  
-| (fm.and p q) := 
-  by {apply and.intro, apply ldq_qfree, apply ldq_qfree} 
-| (fm.or p q) := 
-  by {apply and.intro, apply ldq_qfree, apply ldq_qfree} 
-| (fm.not p) := 
-  by {unfold lift_dnf_qe, apply ldq_qfree}
-| (fm.ex p) := 
-  begin
-    unfold lift_dnf_qe, apply disj_qfree, 
-    unfold qelim, intro l, 
-    apply cases_and_o qfree, trivial, 
-    apply H, apply allp_filter,     
-    apply atoms_conj_qfree, 
-    unfold qfree, apply and.intro, apply H, 
-    apply allp_filter, apply atoms_conj_qfree 
-  end
-
-lemma foo (Q : list β → α → Prop) (a : α) : ∀ (bss : list (list β)), 
-  list.map (λ bs, Q bs a) bss = list.map (λ (P : α → Prop), P a) (list.map Q bss)  
-| [] := eq.refl _
-| (bs::bss) := by simp 
-
 lemma exp_I_list_conj [atom_type α β] (xs : list β) : ∀ (ps : list (fm α)),
 I (list_conj ps) xs = all_true (list.map (λ p, I p xs) ps)  
 | [] := 
@@ -108,6 +26,198 @@ I (list_conj ps) xs = all_true (list.map (λ p, I p xs) ps)
     rewrite exp_I_list_conj, intros q Hq, 
     apply H, apply or.inr, apply Hq 
   end
+
+def qe_prsv (β : Type) [atom_type α β] (qe : list α → fm α) (as : list α) : Prop := 
+  ∀ (bs : list β), ((I (qe as) bs) ↔ (∃ x, allp (val (x::bs)) as))
+
+/- 
+Requires : qe takes a list of atoms that are all dependent on 0-variable,
+  and returns formula which (1) does not contain the 0-variable, and 
+  (2) is equivalent to the conjunction of input list.
+-/
+def qelim (β) [atom_type α β] (qe : list α → fm α) (as : list α) : fm α :=
+  and_o 
+    (qe (@list.filter _ (dep0 β) (dec_dep0 _ _) as)) 
+    (list_conj (list.map (λ (a : α), A' (decr β a)) (@list.filter _ (λ a, ¬ (dep0 β a)) 
+      (begin 
+         intro a, cases (dec_dep0 _ _ a) with H H, 
+         apply decidable.is_true H, 
+         apply decidable.is_false (not_not_intro H)
+       end) as)))
+  
+variable (nm : α → Prop)
+      
+lemma qelim_prsv [atom_type α β] {qe} 
+  (hqe : ∀ as, allp (dep0 β) as → allp (normal β) as → qe_prsv β qe as)
+  {as : list α} {hr : allp (normal β) as} (bs : list β) : 
+  (I (qelim β qe as) bs) ↔ (∃ b, allp (val (b::bs)) as) := 
+begin
+  apply iff.intro; intro h,
+
+  unfold qelim at h, 
+  rewrite exp_I_and_o at h, cases h with h1 h2,
+  rewrite hqe at h1, cases h1 with b h1, 
+  existsi b, intros a ha,
+  cases (atom_type.dec_dep0 _ β a) with hd hd,
+  rewrite exp_I_list_conj at h2, 
+  rewrite map_compose at h2,
+  rewrite iff.symm (decr_prsv α β),
+  apply h2, apply mem_map_of_mem,
+  apply mem_filter_of_pred_and_mem, 
+  apply hd, apply ha, apply hd, 
+  apply h1, apply mem_filter_of_pred_and_mem,
+  apply hd, apply ha, apply allp_filter_cond,
+  apply allp_filter_of_allp, apply hr,
+
+  cases h with b hb, unfold qelim, 
+  rewrite exp_I_and_o, apply and.intro, 
+  rewrite hqe, existsi b, 
+  apply allp_filter_of_allp, apply hb,
+  apply allp_filter_cond, 
+  apply allp_filter_of_allp, apply hr, 
+  rewrite exp_I_list_conj, intros p hp,
+  cases (ex_arg_of_mem_map hp) with q hq,
+  clear hp, simp at hq, cases hq with hq1 hq2, 
+  subst hq1, cases (ex_arg_of_mem_map hq2) with x hx,
+  cases hx with hx1 hx2, simp at hx2, subst hx2, 
+  unfold I, unfold interp, rewrite decr_prsv, 
+  apply hb, apply mem_of_mem_filter, apply hx1, 
+  apply pred_of_mem_filter_pred hx1
+end
+
+lemma fnormal_conj_of_allp_fnormal [atom_type α β] : 
+  ∀ (ps : list (fm α)), allp (fnormal β) ps → fnormal β (list_conj ps) 
+| [] hnm := by unfold list_conj 
+| (p::ps) hnm := 
+  begin
+    unfold list_conj, 
+    apply cases_and_o, trivial,
+    apply hnm, apply or.inl rfl,
+    apply fnormal_conj_of_allp_fnormal,
+    apply allp_of_allp_cons hnm, 
+    unfold fnormal, apply and.intro, 
+    apply hnm, apply or.inl rfl,
+    apply fnormal_conj_of_allp_fnormal,
+    apply allp_of_allp_cons hnm 
+  end 
+
+lemma fnormal_disj_of_allp_fnormal [atom_type α β] : 
+  ∀ (ps : list (fm α)), allp (fnormal β) ps → fnormal β (list_disj ps) 
+| [] hnm := by unfold list_disj 
+| (p::ps) hnm := 
+  begin
+    unfold list_disj, 
+    apply cases_or_o, trivial,
+    apply hnm, apply or.inl rfl,
+    apply fnormal_disj_of_allp_fnormal,
+    apply allp_of_allp_cons hnm, 
+    unfold fnormal, apply and.intro, 
+    apply hnm, apply or.inl rfl,
+    apply fnormal_disj_of_allp_fnormal,
+    apply allp_of_allp_cons hnm 
+  end 
+
+meta def qelim_prsv_normal_tac :=
+`[apply fnormal_conj_of_allp_fnormal,
+  intros p hp, rewrite exp_mem_map at hp,
+  cases hp with a ha, cases ha with ha1 ha2,
+  subst ha2, apply atom_type.decr_prsv_normal,
+  apply hnm, apply mem_of_mem_filter ha1,
+  apply pred_of_mem_filter_pred ha1]
+
+lemma qelim_prsv_normal [atom_type α β] {qe : list α → fm α}
+  {hqe : ∀ (as : list α), allp (normal β) as → fnormal β (qe as)}  
+  {as : list α} (hnm : allp (normal β) as) : fnormal β (qelim β qe as) := 
+begin
+  unfold qelim, apply cases_and_o,
+  trivial, apply hqe, 
+  apply allp_filter_of_allp hnm,
+  qelim_prsv_normal_tac,
+  unfold fnormal, apply and.intro, 
+  apply hqe, apply allp_filter_of_allp hnm,
+  qelim_prsv_normal_tac
+end
+
+
+
+def lift_dnf_qe (β : Type) [atom_type α β] (qe : list α → fm α) : fm α → fm α 
+| (fm.true α) := ⊤'
+| (fm.false α) := ⊥'
+| (fm.atom a) := A' a
+| (fm.and p q) := (lift_dnf_qe p) ∧' (lift_dnf_qe q)
+| (fm.or p q) := (lift_dnf_qe p) ∨' (lift_dnf_qe q)
+| (fm.not p) := ¬' (lift_dnf_qe p) 
+| (fm.ex p) := dnf_to_fm (dnf (@nnf _ β _ $ lift_dnf_qe p)) (@qelim _ β _ @qe)
+
+lemma atoms_conj_qfree [atom_type α β] : ∀ (as : list α), qfree (list_conj (list.map (λ (a : α), A' decr β a) as )) 
+| [] := trivial
+| (a::as) := 
+  begin 
+    unfold list.map, unfold list_conj, 
+    apply cases_and_o, trivial, trivial,
+    apply atoms_conj_qfree, unfold qfree, 
+    apply and.intro trivial,
+    apply atoms_conj_qfree
+  end
+
+meta def ldq_normal_tac := 
+`[unfold fnormal at hnm, cases hnm with hnmp hnmq,
+  unfold lift_dnf_qe, unfold fnormal,
+  apply and.intro; apply ldq_normal; assumption]
+
+
+lemma ldq_normal [atom_type α β] (qe : list α → fm α)  
+  (hqe : ∀ (as : list α), allp (normal β) as → fnormal β (qe as)) :
+  ∀ p, fnormal β p → fnormal β (lift_dnf_qe β qe p) 
+| (fm.true α) hnm := trivial
+| (fm.false α) hnm := trivial
+| (fm.atom a) hnm := hnm 
+| (fm.and p q) hnm := by ldq_normal_tac
+| (fm.or p q) hnm := by ldq_normal_tac
+| (fm.not p) hnm := 
+  begin
+    unfold lift_dnf_qe, unfold fnormal,
+    apply ldq_normal, apply hnm
+  end
+| (fm.ex p) hnm := 
+  begin
+    unfold lift_dnf_qe, unfold dnf_to_fm,
+    apply fnormal_disj_of_allp_fnormal,
+    intros a ha, rewrite exp_mem_map at ha,
+    cases ha with as has, cases has with has1 has2,
+    subst has2, apply qelim_prsv_normal, apply hqe,
+    apply dnf_prsv_normal, apply nnf_prsv_normal, 
+    apply ldq_normal, unfold fnormal at hnm, apply hnm,
+    apply has1
+  end
+
+lemma ldq_qfree [atom_type α β] (qe : list α → fm α)  
+  (H : ∀ (l : list α), allp (dep0 β) l → qfree (qe l)) :
+  ∀ (p : fm α), qfree (lift_dnf_qe β qe p)  
+| (fm.true α) := trivial
+| (fm.false α) := trivial
+| (fm.atom a) := trivial  
+| (fm.and p q) := 
+  by {apply and.intro, apply ldq_qfree, apply ldq_qfree} 
+| (fm.or p q) := 
+  by {apply and.intro, apply ldq_qfree, apply ldq_qfree} 
+| (fm.not p) := 
+  by {unfold lift_dnf_qe, apply ldq_qfree}
+| (fm.ex p) := 
+  begin
+    unfold lift_dnf_qe, apply disj_qfree, 
+    unfold qelim, intro l, 
+    apply cases_and_o qfree, trivial, 
+    apply H, apply allp_filter_cond,     
+    apply atoms_conj_qfree, 
+    unfold qfree, apply and.intro, apply H, 
+    apply allp_filter_cond, apply atoms_conj_qfree 
+  end
+
+-- lemma foo (Q : list β → α → Prop) (a : α) : ∀ (bss : list (list β)), 
+  -- list.map (λ bs, Q bs a) bss = list.map (λ (P : α → Prop), P a) (list.map Q bss)  
+-- | [] := eq.refl _
+-- | (bs::bss) := by simp 
 
 lemma exp_I_list_disj [atom_type α β] (xs : list β) : ∀ (ps : list (fm α)),
 I (list_disj ps) xs ↔ disj_list (list.map (λ p, I p xs) ps)  
@@ -152,6 +262,42 @@ lemma dist_ex_disj_list [atom_type α β] : ∀ (ps : list (β → Prop)),
 
 instance atom_type_to_dec_eq [atom_type α β] : decidable_eq α := atom_type.dec_eq α β 
 
+lemma ldq_prsv_gen_ex [atom_type α β] 
+(qe : list α → fm α)
+(hqep : ∀ (as : list α), allp (dep0 β) as → allp (normal β) as → qe_prsv β qe as)
+(p : fm α) (hpn : fnormal β p) (hpnq : nqfree p) (bs : list β) : 
+  some_true (list.map (λ (x : list α), I (qelim β qe x) bs) (dnf p)) 
+  ↔ ∃ (b : β), I p (b :: bs) := 
+begin
+  apply iff.intro; intro h,
+
+  cases h with q hq, cases hq with hq1 hq2,
+  cases (ex_arg_of_mem_map hq1) with as has,
+  cases has with has1 has2, simp at has2,
+  subst has2, 
+  rewrite (@qelim_prsv α β) at hq2,
+  cases hq2 with b hb, existsi b, 
+  rewrite iff.symm dnf_prsv,
+  existsi (allp (val (b :: bs)) as),
+  apply and.intro, 
+  apply mem_map_of_mem, apply has1, 
+  apply hb, apply hpnq, apply hqep,
+  apply dnf_prsv_normal,
+  apply hpn,
+  
+  apply has1, cases h with b hb, 
+  rewrite iff.symm dnf_prsv at hb, 
+  cases hb with q hq, cases hq with hq1 hq2,
+  cases (ex_arg_of_mem_map hq1) with as has,
+  cases has with has1 has2, subst has2, 
+  existsi (I (qelim β qe as) bs), 
+  apply and.intro, apply mem_map_of_mem,
+  apply has1, rewrite (@qelim_prsv _ β), 
+  existsi b, apply hq2, apply hqep, 
+  apply dnf_prsv_normal,
+  apply hpn, apply has1, apply hpnq
+end
+
 meta def ldq_prsv_core_aux := 
 `[repeat {rewrite ldq_prsv_gen}, 
   intros a ha, 
@@ -161,68 +307,37 @@ meta def ldq_prsv_core_aux :=
   apply hp, unfold atoms, 
   apply mem_union_of_mem_left, apply ha]
 
-lemma ldq_prsv_gen_ex [atom_type α β] 
-(qe : list α → fm α)
-(hqf : ∀ (as : list α), allp (dep0 β) as → qfree (qe as))
-(r : α → Prop)
-(hqe : ∀ (as : list α), allp (dep0 β) as → allp r as → qe_prsv β qe as)
-(p : fm α)
-(hnqf : nqfree p)
-(bs : list β)
-: some_true (list.map (λ (x : list α), I (qelim β qe x) bs) (dnf p)) ↔
-    ∃ (b : β), I p (b :: bs) := 
-begin
-  apply iff.intro; intro h,
-
-  cases h with q hq, cases hq with hq1 hq2,
-  cases (ex_arg_of_mem_map hq1) with as has,
-  cases has with has1 has2, simp at has2,
-  subst has2, rewrite qelim_prsv at hq2,
-  cases hq2 with b hb, existsi b, 
-  rewrite iff.symm dnf_prsv,
-  existsi (allp (val (b :: bs)) as),
-  apply and.intro, 
-  apply mem_map_of_mem, apply has1, 
-  apply hb, apply hnqf, apply hqe,
-
-  cases h with b hb, 
-  rewrite iff.symm dnf_prsv at hb, 
-  cases hb with q hq, cases hq with hq1 hq2,
-  cases (ex_arg_of_mem_map hq1) with as has,
-  cases has with has1 has2, subst has2, 
-  existsi (I (qelim β qe as) bs), 
-  apply and.intro, apply mem_map_of_mem,
-  apply has1, rewrite qelim_prsv, 
-  existsi b, apply hq2, apply hqe, apply hnqf
-end
-
-lemma ldq_prsv_gen [atom_type α β] (qe : list α → fm α)  
-  (hqf : ∀ as, allp (dep0 β) as → qfree (qe as)) 
-  (r : α → Prop) 
-  (hr : ∀ as, allp (dep0 β) as → allp r as → fnormal β (qe as)) 
-  (he : ∀ as, allp (dep0 β) as → allp r as → qe_prsv β qe as) : 
-  ∀ p, allp r (atoms p) → ∀ (bs : list β), I (lift_dnf_qe β qe p) bs ↔ I p bs 
+lemma ldq_prsv_gen [atom_type α β] 
+  (qe : list α → fm α)  
+  (hqef : ∀ as, allp (dep0 β) as → qfree (qe as)) 
+  (hqen : ∀ as, allp (normal β) as → fnormal β (qe as))
+  (hqep : ∀ as, allp (dep0 β) as → allp (normal β) as → qe_prsv β qe as) : 
+  ∀ p, fnormal β p → ∀ (bs : list β), I (lift_dnf_qe β qe p) bs ↔ I p bs 
 | ⊤' _ bs := iff.refl _
 | ⊥' _ bs := iff.refl _
 | (A' a) hp bs := iff.refl _
 | (p ∧' q) hp bs := 
   begin
+    cases hp with hp1 hp2, 
     unfold lift_dnf_qe,
     repeat {rewrite exp_I_and}, 
-    ldq_prsv_core_aux
+    repeat {rewrite ldq_prsv_gen}, 
+    apply hp2, apply hp1
   end
 | (p ∨' q) hp bs := 
   begin
+    cases hp with hp1 hp2, 
     unfold lift_dnf_qe,
     repeat {rewrite exp_I_or}, 
-    ldq_prsv_core_aux
+    repeat {rewrite ldq_prsv_gen}, 
+    apply hp2, apply hp1
   end
 | (¬' p) hp bs := 
   begin
     unfold lift_dnf_qe,
     repeat {rewrite exp_I_not}, 
     repeat {rewrite ldq_prsv_gen}, 
-    intros a ha, apply hp, apply ha
+    apply hp 
   end
 | (∃' p) hp bs := 
   calc 
@@ -231,16 +346,18 @@ lemma ldq_prsv_gen [atom_type α β] (qe : list α → fm α)
         begin
           unfold lift_dnf_qe, unfold dnf_to_fm,
           rewrite exp_I_list_disj_alt,
-          rewrite map_compose, apply ldq_prsv_gen_ex,
-          apply hqf, apply he, apply nnf_nqfree, 
-          apply ldq_qfree, apply hqf
+          rewrite map_compose, apply
+          (@ldq_prsv_gen_ex α β), apply hqep,
+          apply nnf_prsv_normal, apply ldq_normal, 
+          apply hqen, apply hp, apply nnf_nqfree, 
+          apply ldq_qfree, apply hqef
         end
   ... ↔ I (∃' p) bs : 
         begin
           rewrite exp_I_ex, apply ex_iff_ex,
           intro b, rewrite nnf_prsv,
           rewrite ldq_prsv_gen, apply hp,
-          apply ldq_qfree, apply hqf
+          apply ldq_qfree, apply hqef
         end 
 
 #exit
@@ -327,5 +444,5 @@ lemma ldq_prsv [HA : atom_type α β] (qe : list α → fm α)
     apply mem_filter_of_pred_and_mem, 
     apply HD, apply Ha, apply HD, 
     apply Hb, apply mem_filter_of_pred_and_mem,
-    apply HD, apply Ha, apply allp_filter,
+    apply HD, apply Ha, apply allp_filter_cond,
   end
